Let the values $t, r, k$ be the threshold, ratio and knee parameters of a compressor. For a softknee compressor curve, we want to fit a pentic of the form:
\begin{equation}
 f(x) = a_5 x^5 + a_4 x^4 + a_3 x^3 + a_2 x^2 + a_1 x + a_0
\end{equation}
with first and second derivatives:
\begin{equation}
 f'(x) = 5 a_5 x^4 + 4 a_4 x^3 + 3 a_3 x^2 + 2 a_2 x +  a_1
 \qquad
 f''(x) = 20 a_5 x^3 + 12 a_4 x^2 + 6 a_3 x + 2 a_2
\end{equation}
between the two points:
\begin{equation}
 x_1 = t-\frac{k}{2}, \qquad y_1 = t-\frac{k}{2}
\end{equation}
\begin{equation}
 x_2 = t+\frac{k}{2}, \qquad y_2 = t + \frac{k}{2r}
\end{equation}
with first and second derivatives:
\begin{equation}
 y_1' = 1, \qquad y_2' = \frac{1}{r}, \qquad y_1'' = 0, \qquad y_2'' = 0
\end{equation}
Let $c = \frac{k}{2}$. Then, these condidtions give rise to the system of equations for the 6 unknown polynomial coefficients:
\begin{equation}
 \begin{aligned}
 t-c           &= a_5 (t-c)^5 + a_4 (t-c)^4 + a_3 (t-c)^3 + a_2 (t-c)^2 + a_1 (t-c) + a_0  \\
 t+\frac{c}{r} &= a_5 (t+c)^5 + a_4 (t+c)^4 + a_3 (t+c)^3 + a_2 (t+c)^2 + a_1 (t+c) + a_0  \\
 1             &= 5 a_5 (t-c)^4 + 4 a_4 (t-c)^3 + 3 a_3 (t-c)^2 + 2 a_2 (t-c) +  a_1   \\
 \frac{1}{r}   &= 5 a_5 (t+c)^4 + 4 a_4 (t+c)^3 + 3 a_3 (t+c)^2 + 2 a_2 (t+c) +  a_1   \\
 0             &= 20 a_5 (t-c)^3 + 12 a_4 (t-c)^2 + 6 a_3 (t-c) + 2 a_2      \\
 0             &= 20 a_5 (t+c)^3 + 12 a_4 (t+c)^2 + 6 a_3 (t+c) + 2 a_2     
 \end{aligned}
\end{equation}
passing the following lines to maxima:
\begin{verbatim}
e1: t-c   = a5*(t-c)^5 + a4*(t-c)^4 + a3*(t-c)^3 + a2*(t-c)^2 + a1*(t-c) + a0;
e2: t+c/r = a5*(t+c)^5 + a4*(t+c)^4 + a3*(t+c)^3 + a2*(t+c)^2 + a1*(t+c) + a0;
e3: 1     = 5*a5*(t-c)^4 + 4*a4*(t-c)^3 + 3*a3*(t-c)^2 + 2*a2*(t-c) + a1;
e4: 1/r   = 5*a5*(t+c)^4 + 4*a4*(t+c)^3 + 3*a3*(t+c)^2 + 2*a2*(t+c) +  a1;
e5: 0     = 20*a5*(t-c)^3 + 12*a4*(t-c)^2 + 6*a3*(t-c) + 2*a2;
e6: 0     = 20*a5*(t+c)^3 + 12*a4*(t+c)^2 + 6*a3*(t+c) + 2*a2;
solve([e1,e2,e3,e4,e5,e6],[a0,a1,a2,a3,a4,a5]);
\end{verbatim}
yields the solution:
\begin{equation}
 \mathrm{a_0}=\frac{\left(r-1\right)\,t^4+c^2\,\left(6-6\,r\right)\,t^2+c^3\,\left(8\,r-8\right)\,t+c^4\,\left(3-3\,r\right)}{16\,c^3\,r}
\end{equation}
\begin{equation}
 \mathrm{a_1}=-\frac{\left(r-1\right)\,t^3+c^2\,\left(3-3\,r\right)\,t+c^3\,\left(-2\,r-2\right)}{4\,c^3\,r}, \qquad
 \mathrm{a_2}=\frac{\left(3\,r-3\right)\,t^2+c^2\,\left(3-3\,r\right)}{8\,c^3\,r} 
\end{equation}
\begin{equation}
 \mathrm{a_3}=-\frac{\left(r-1\right)\,t}{4\,c^3\,r}, \qquad
 \mathrm{a_4}=\frac{r-1}{16\,c^3\,r},                 \qquad
 \mathrm{a_5}=0  
\end{equation}

% original maxima output:
%\left[ \left[ \mathrm{a\_0}=\ifrac{\left(r-1\right)\,t^4+c^2\,\left(6-6\,r\right)\,t^2+c^3\,\left(8\,r-8\right)\,t+c^4\,\left(3-3\,r\right)}{16\,c^3\,r} , \linebreak[0]\mathrm{a\_1}=-\ifrac{\left(r-1\right)\,t^3+c^2\,\left(3-3\,r\right)\,t+c^3\,\left(-2\,r-2\right)}{4\,c^3\,r} , \linebreak[0]\mathrm{a\_2}=\ifrac{\left(3\,r-3\right)\,t^2+c^2\,\left(3-3\,r\right)}{8\,c^3\,r} , \linebreak[0]\mathrm{a\_3}=-\ifrac{\left(r-1\right)\,t}{4\,c^3\,r} , \linebreak[0]\mathrm{a\_4}=\ifrac{r-1}{16\,c^3\,r} , \linebreak[0]\mathrm{a\_5}=0 \right]  \right] 



















